rules/single-line-swap/single-line-swap.yul
@@ -1,17 +1,18 @@
+IR:
 
 /// @use-src 0:"Ao.sol"
-object "Ao_49" {
+object "Ao_60" {
     code {
-        /// @src 0:97:569  "contract Ao {..."
+        /// @src 0:524:1126  "contract Ao {..."
         mstore(64, memoryguard(128))
         if callvalue() { revert_error_ca66f745a3ce8ff40e2ccaf1ad45db7774001b90d25810abd9040049be7bf4bb() }
 
-        constructor_Ao_49()
+        constructor_Ao_60()
 
         let _1 := allocate_unbounded()
-        codecopy(_1, dataoffset("Ao_49_deployed"), datasize("Ao_49_deployed"))
+        codecopy(_1, dataoffset("Ao_60_deployed"), datasize("Ao_60_deployed"))
 
-        return(_1, datasize("Ao_49_deployed"))
+        return(_1, datasize("Ao_60_deployed"))
 
         function allocate_unbounded() -> memPtr {
             memPtr := mload(64)
@@ -21,19 +22,19 @@ object "Ao_49" {
             revert(0, 0)
         }
 
-        /// @src 0:97:569  "contract Ao {..."
-        function constructor_Ao_49() {
+        /// @src 0:524:1126  "contract Ao {..."
+        function constructor_Ao_60() {
 
-            /// @src 0:97:569  "contract Ao {..."
+            /// @src 0:524:1126  "contract Ao {..."
 
         }
-        /// @src 0:97:569  "contract Ao {..."
+        /// @src 0:524:1126  "contract Ao {..."
 
     }
     /// @use-src 0:"Ao.sol"
-    object "Ao_49_deployed" {
+    object "Ao_60_deployed" {
         code {
-            /// @src 0:97:569  "contract Ao {..."
+            /// @src 0:524:1126  "contract Ao {..."
             mstore(64, memoryguard(128))
 
             if iszero(lt(calldatasize(), 4))
@@ -45,21 +46,28 @@ object "Ao_49" {
                 {
                     // f(uint256,uint256)
 
-                    external_fun_f_48()
+                    external_fun_f_59()
                 }
 
-                case 0x2113522a
+                case 0x51973ec9
                 {
-                    // lastCaller()
+                    // log()
 
-                    external_fun_lastCaller_3()
+                    external_fun_log_7()
                 }
 
-                case 0x2ddbd13a
+                case 0x61bc221a
                 {
-                    // total()
+                    // counter()
 
-                    external_fun_total_5()
+                    external_fun_counter_3()
+                }
+
+                case 0x890eba68
+                {
+                    // flag()
+
+                    external_fun_flag_5()
                 }
 
                 default {}
@@ -135,11 +143,11 @@ object "Ao_49" {
 
             }
 
-            function external_fun_f_48() {
+            function external_fun_f_59() {
 
                 if callvalue() { revert_error_ca66f745a3ce8ff40e2ccaf1ad45db7774001b90d25810abd9040049be7bf4bb() }
                 let param_0, param_1 :=  abi_decode_tuple_t_uint256t_uint256(4, calldatasize())
-                let ret_0, ret_1 :=  fun_f_48(param_0, param_1)
+                let ret_0, ret_1 :=  fun_f_59(param_0, param_1)
                 let memPos := allocate_unbounded()
                 let memEnd := abi_encode_tuple_t_uint256_t_uint256__to_t_uint256_t_uint256__fromStack(memPos , ret_0, ret_1)
                 return(memPos, sub(memEnd, memPos))
@@ -158,61 +166,6 @@ object "Ao_49" {
 
             }
 
-            function cleanup_from_storage_t_address(value) -> cleaned {
-                cleaned := and(value, 0xffffffffffffffffffffffffffffffffffffffff)
-            }
-
-            function extract_from_storage_value_dynamict_address(slot_value, offset) -> value {
-                value := cleanup_from_storage_t_address(shift_right_unsigned_dynamic(mul(offset, 8), slot_value))
-            }
-
-            function read_from_storage_split_dynamic_t_address(slot, offset) -> value {
-                value := extract_from_storage_value_dynamict_address(sload(slot), offset)
-
-            }
-
-            /// @ast-id 3
-            /// @src 0:115:140  "address public lastCaller"
-            function getter_fun_lastCaller_3() -> ret {
-
-                let slot := 0
-                let offset := 0
-
-                ret := read_from_storage_split_dynamic_t_address(slot, offset)
-
-            }
-            /// @src 0:97:569  "contract Ao {..."
-
-            function cleanup_t_uint160(value) -> cleaned {
-                cleaned := and(value, 0xffffffffffffffffffffffffffffffffffffffff)
-            }
-
-            function cleanup_t_address(value) -> cleaned {
-                cleaned := cleanup_t_uint160(value)
-            }
-
-            function abi_encode_t_address_to_t_address_fromStack(value, pos) {
-                mstore(pos, cleanup_t_address(value))
-            }
-
-            function abi_encode_tuple_t_address__to_t_address__fromStack(headStart , value0) -> tail {
-                tail := add(headStart, 32)
-
-                abi_encode_t_address_to_t_address_fromStack(value0,  add(headStart, 0))
-
-            }
-
-            function external_fun_lastCaller_3() {
-
-                if callvalue() { revert_error_ca66f745a3ce8ff40e2ccaf1ad45db7774001b90d25810abd9040049be7bf4bb() }
-                abi_decode_tuple_(4, calldatasize())
-                let ret_0 :=  getter_fun_lastCaller_3()
-                let memPos := allocate_unbounded()
-                let memEnd := abi_encode_tuple_t_address__to_t_address__fromStack(memPos , ret_0)
-                return(memPos, sub(memEnd, memPos))
-
-            }
-
             function cleanup_from_storage_t_uint256(value) -> cleaned {
                 cleaned := value
             }
@@ -226,17 +179,17 @@ object "Ao_49" {
 
             }
 
-            /// @ast-id 5
-            /// @src 0:146:166  "uint256 public total"
-            function getter_fun_total_5() -> ret {
+            /// @ast-id 7
+            /// @src 0:596:614  "uint256 public log"
+            function getter_fun_log_7() -> ret {
 
-                let slot := 1
+                let slot := 2
                 let offset := 0
 
                 ret := read_from_storage_split_dynamic_t_uint256(slot, offset)
 
             }
-            /// @src 0:97:569  "contract Ao {..."
+            /// @src 0:524:1126  "contract Ao {..."
 
             function abi_encode_tuple_t_uint256__to_t_uint256__fromStack(headStart , value0) -> tail {
                 tail := add(headStart, 32)
@@ -245,13 +198,87 @@ object "Ao_49" {
 
             }
 
-            function external_fun_total_5() {
+            function external_fun_log_7() {
 
                 if callvalue() { revert_error_ca66f745a3ce8ff40e2ccaf1ad45db7774001b90d25810abd9040049be7bf4bb() }
                 abi_decode_tuple_(4, calldatasize())
-                let ret_0 :=  getter_fun_total_5()
+                let ret_0 :=  getter_fun_log_7()
                 let memPos := allocate_unbounded()
                 let memEnd := abi_encode_tuple_t_uint256__to_t_uint256__fromStack(memPos , ret_0)
+                return(memPos, sub(memEnd, memPos))
+
+            }
+
+            /// @ast-id 3
+            /// @src 0:542:564  "uint256 public counter"
+            function getter_fun_counter_3() -> ret {
+
+                let slot := 0
+                let offset := 0
+
+                ret := read_from_storage_split_dynamic_t_uint256(slot, offset)
+
+            }
+            /// @src 0:524:1126  "contract Ao {..."
+
+            function external_fun_counter_3() {
+
+                if callvalue() { revert_error_ca66f745a3ce8ff40e2ccaf1ad45db7774001b90d25810abd9040049be7bf4bb() }
+                abi_decode_tuple_(4, calldatasize())
+                let ret_0 :=  getter_fun_counter_3()
+                let memPos := allocate_unbounded()
+                let memEnd := abi_encode_tuple_t_uint256__to_t_uint256__fromStack(memPos , ret_0)
+                return(memPos, sub(memEnd, memPos))
+
+            }
+
+            function cleanup_from_storage_t_bool(value) -> cleaned {
+                cleaned := and(value, 0xff)
+            }
+
+            function extract_from_storage_value_dynamict_bool(slot_value, offset) -> value {
+                value := cleanup_from_storage_t_bool(shift_right_unsigned_dynamic(mul(offset, 8), slot_value))
+            }
+
+            function read_from_storage_split_dynamic_t_bool(slot, offset) -> value {
+                value := extract_from_storage_value_dynamict_bool(sload(slot), offset)
+
+            }
+
+            /// @ast-id 5
+            /// @src 0:570:590  "bool     public flag"
+            function getter_fun_flag_5() -> ret {
+
+                let slot := 1
+                let offset := 0
+
+                ret := read_from_storage_split_dynamic_t_bool(slot, offset)
+
+            }
+            /// @src 0:524:1126  "contract Ao {..."
+
+            function cleanup_t_bool(value) -> cleaned {
+                cleaned := iszero(iszero(value))
+            }
+
+            function abi_encode_t_bool_to_t_bool_fromStack(value, pos) {
+                mstore(pos, cleanup_t_bool(value))
+            }
+
+            function abi_encode_tuple_t_bool__to_t_bool__fromStack(headStart , value0) -> tail {
+                tail := add(headStart, 32)
+
+                abi_encode_t_bool_to_t_bool_fromStack(value0,  add(headStart, 0))
+
+            }
+
+            function external_fun_flag_5() {
+
+                if callvalue() { revert_error_ca66f745a3ce8ff40e2ccaf1ad45db7774001b90d25810abd9040049be7bf4bb() }
+                abi_decode_tuple_(4, calldatasize())
+                let ret_0 :=  getter_fun_flag_5()
+                let memPos := allocate_unbounded()
+                let memEnd := abi_encode_tuple_t_bool__to_t_bool__fromStack(memPos , ret_0)
                 return(memPos, sub(memEnd, memPos))
 
             }
@@ -264,43 +291,32 @@ object "Ao_49" {
                 ret := 0
             }
 
-            function shift_left_0(value) -> newValue {
+            function shift_right_0_unsigned(value) -> newValue {
                 newValue :=
 
-                shl(0, value)
+                shr(0, value)
 
             }
 
-            function update_byte_slice_20_shift_0(value, toInsert) -> result {
-                let mask := 0xffffffffffffffffffffffffffffffffffffffff
-                toInsert := shift_left_0(toInsert)
-                value := and(value, not(mask))
-                result := or(value, and(toInsert, mask))
+            function extract_from_storage_value_offset_0t_uint256(slot_value) -> value {
+                value := cleanup_from_storage_t_uint256(shift_right_0_unsigned(slot_value))
+            }
+
+            function read_from_storage_split_offset_0_t_uint256(slot) -> value {
+                value := extract_from_storage_value_offset_0t_uint256(sload(slot))
+
+            }
+
+            function cleanup_t_rational_1_by_1(value) -> cleaned {
+                cleaned := value
             }
 
             function identity(value) -> ret {
                 ret := value
             }
 
-            function convert_t_uint160_to_t_uint160(value) -> converted {
-                converted := cleanup_t_uint160(identity(cleanup_t_uint160(value)))
-            }
-
-            function convert_t_uint160_to_t_address(value) -> converted {
-                converted := convert_t_uint160_to_t_uint160(value)
-            }
-
-            function convert_t_address_to_t_address(value) -> converted {
-                converted := convert_t_uint160_to_t_address(value)
-            }
-
-            function prepare_store_t_address(value) -> ret {
-                ret := value
-            }
-
-            function update_storage_value_offset_0t_address_to_t_address(slot, value_0) {
-                let convertedValue_0 := convert_t_address_to_t_address(value_0)
-                sstore(slot, update_byte_slice_20_shift_0(sload(slot), prepare_store_t_address(convertedValue_0)))
+            function convert_t_rational_1_by_1_to_t_uint256(value) -> converted {
+                converted := cleanup_t_uint256(identity(cleanup_t_rational_1_by_1(value)))
             }
 
             function panic_error_0x11() {
@@ -315,6 +331,13 @@ object "Ao_49" {
                 sum := add(x, y)
 
                 if gt(x, sum) { panic_error_0x11() }
+
+            }
+
+            function shift_left_0(value) -> newValue {
+                newValue :=
+
+                shl(0, value)
 
             }
 
@@ -338,78 +361,115 @@ object "Ao_49" {
                 sstore(slot, update_byte_slice_32_shift_0(sload(slot), prepare_store_t_uint256(convertedValue_0)))
             }
 
-            /// @ast-id 48
-            /// @src 0:173:567  "function f(uint256 x, uint256 y) external returns (uint256, uint256) {..."
-            function fun_f_48(var_x_7, var_y_9) -> var__12, var__14 {
-                /// @src 0:224:231  "uint256"
+            function update_byte_slice_1_shift_0(value, toInsert) -> result {
+                let mask := 255
+                toInsert := shift_left_0(toInsert)
+                value := and(value, not(mask))
+                result := or(value, and(toInsert, mask))
+            }
+
+            function convert_t_bool_to_t_bool(value) -> converted {
+                converted := cleanup_t_bool(value)
+            }
+
+            function prepare_store_t_bool(value) -> ret {
+                ret := value
+            }
+
+            function update_storage_value_offset_0t_bool_to_t_bool(slot, value_0) {
+                let convertedValue_0 := convert_t_bool_to_t_bool(value_0)
+                sstore(slot, update_byte_slice_1_shift_0(sload(slot), prepare_store_t_bool(convertedValue_0)))
+            }
+
+            /// @ast-id 59
+            /// @src 0:621:1124  "function f(uint256 x, uint256 y) external returns (uint256, uint256) {..."
+            function fun_f_59(var_x_9, var_y_11) -> var__14, var__16 {
+                /// @src 0:672:679  "uint256"
                 let zero_t_uint256_1 := zero_value_for_split_t_uint256()
-                var__12 := zero_t_uint256_1
-                /// @src 0:233:240  "uint256"
+                var__14 := zero_t_uint256_1
+                /// @src 0:681:688  "uint256"
                 let zero_t_uint256_2 := zero_value_for_split_t_uint256()
-                var__14 := zero_t_uint256_2
+                var__16 := zero_t_uint256_2
 
-                /// @src 0:307:317  "msg.sender"
-                let expr_18 := caller()
-                /// @src 0:294:317  "lastCaller = msg.sender"
-                update_storage_value_offset_0t_address_to_t_address(0x00, expr_18)
-                let expr_19 := expr_18
-                /// @src 0:343:344  "x"
-                let _3 := var_x_7
-                let expr_23 := _3
-                /// @src 0:328:344  "uint256 varA = x"
-                let var_varA_22 := expr_23
-                /// @src 0:369:370  "y"
-                let _4 := var_y_9
-                let expr_27 := _4
-                /// @src 0:354:370  "uint256 varB = y"
-                let var_varB_26 := expr_27
-                /// @src 0:448:452  "varB"
-                let _5 := var_varB_26
-                let expr_32 := _5
-                /// @src 0:447:459  "(varB, varA)"
-                let expr_34_component_1 := expr_32
-                /// @src 0:454:458  "varA"
-                let _6 := var_varA_22
-                let expr_33 := _6
-                /// @src 0:447:459  "(varB, varA)"
-                let expr_34_component_2 := expr_33
-                /// @src 0:432:459  "(varA, varB) = (varB, varA)"
-                var_varB_26 := expr_34_component_2
-                var_varA_22 := expr_34_component_1
-                /// @src 0:519:523  "varA"
-                let _7 := var_varA_22
-                let expr_38 := _7
-                /// @src 0:526:530  "varB"
-                let _8 := var_varB_26
-                let expr_39 := _8
-                /// @src 0:519:530  "varA + varB"
-                let expr_40 := checked_add_t_uint256(expr_38, expr_39)
+                /// @src 0:733:740  "counter"
+                let _3 := read_from_storage_split_offset_0_t_uint256(0x00)
+                let expr_19 := _3
+                /// @src 0:743:744  "1"
+                let expr_20 := 0x01
+                /// @src 0:733:744  "counter + 1"
+                let expr_21 := checked_add_t_uint256(expr_19, convert_t_rational_1_by_1_to_t_uint256(expr_20))
 
-                /// @src 0:511:530  "total = varA + varB"
-                update_storage_value_offset_0t_uint256_to_t_uint256(0x01, expr_40)
-                let expr_41 := expr_40
-                /// @src 0:549:553  "varA"
-                let _9 := var_varA_22
-                let expr_43 := _9
-                /// @src 0:548:560  "(varA, varB)"
-                let expr_45_component_1 := expr_43
-                /// @src 0:555:559  "varB"
-                let _10 := var_varB_26
-                let expr_44 := _10
-                /// @src 0:548:560  "(varA, varB)"
-                let expr_45_component_2 := expr_44
-                /// @src 0:541:560  "return (varA, varB)"
-                var__12 := expr_45_component_1
-                var__14 := expr_45_component_2
+                /// @src 0:723:744  "counter = counter + 1"
+                update_storage_value_offset_0t_uint256_to_t_uint256(0x00, expr_21)
+                let expr_22 := expr_21
+                /// @src 0:770:771  "x"
+                let _4 := var_x_9
+                let expr_26 := _4
+                /// @src 0:755:771  "uint256 varA = x"
+                let var_varA_25 := expr_26
+                /// @src 0:796:797  "y"
+                let _5 := var_y_11
+                let expr_30 := _5
+                /// @src 0:781:797  "uint256 varB = y"
+                let var_varB_29 := expr_30
+                /// @src 0:870:874  "varB"
+                let _6 := var_varB_29
+                let expr_35 := _6
+                /// @src 0:869:881  "(varB, varA)"
+                let expr_37_component_1 := expr_35
+                /// @src 0:876:880  "varA"
+                let _7 := var_varA_25
+                let expr_36 := _7
+                /// @src 0:869:881  "(varB, varA)"
+                let expr_37_component_2 := expr_36
+                /// @src 0:854:881  "(varA, varB) = (varB, varA)"
+                var_varB_29 := expr_37_component_2
+                var_varA_25 := expr_37_component_1
+                /// @src 0:951:955  "true"
+                let expr_41 := 0x01
+                /// @src 0:944:955  "flag = true"
+                update_storage_value_offset_0t_bool_to_t_bool(0x01, expr_41)
+                let expr_42 := expr_41
+                /// @src 0:1024:1031  "counter"
+                let _8 := read_from_storage_split_offset_0_t_uint256(0x00)
+                let expr_45 := _8
+                /// @src 0:1018:1031  "log = counter"
+                update_storage_value_offset_0t_uint256_to_t_uint256(0x02, expr_45)
+                let expr_46 := expr_45
+                /// @src 0:1076:1083  "counter"
+                let _9 := read_from_storage_split_offset_0_t_uint256(0x00)
+                let expr_49 := _9
+                /// @src 0:1086:1087  "1"
+                let expr_50 := 0x01
+                /// @src 0:1076:1087  "counter + 1"
+                let expr_51 := checked_add_t_uint256(expr_49, convert_t_rational_1_by_1_to_t_uint256(expr_50))
+
+                /// @src 0:1066:1087  "counter = counter + 1"
+                update_storage_value_offset_0t_uint256_to_t_uint256(0x00, expr_51)
+                let expr_52 := expr_51
+                /// @src 0:1106:1110  "varA"
+                let _10 := var_varA_25
+                let expr_54 := _10
+                /// @src 0:1105:1117  "(varA, varB)"
+                let expr_56_component_1 := expr_54
+                /// @src 0:1112:1116  "varB"
+                let _11 := var_varB_29
+                let expr_55 := _11
+                /// @src 0:1105:1117  "(varA, varB)"
+                let expr_56_component_2 := expr_55
+                /// @src 0:1098:1117  "return (varA, varB)"
+                var__14 := expr_56_component_1
+                var__16 := expr_56_component_2
                 leave
 
             }
-            /// @src 0:97:569  "contract Ao {..."
+            /// @src 0:524:1126  "contract Ao {..."
 
         }
 
-        data ".metadata" hex"a26469706673582212207d003eef9a710f724e983b7732646dbb23ae841cf276e96823a22e21a2c3308a64736f6c634300081a0033"
+        data ".metadata" hex"a26469706673582212207a7f962d56260093c8815f6a05ae7d0406e09ebaac36e300a928eadf086f62a664736f6c634300081a0033"
     }
 
 }
+
 
